Lift reaction(s) into type(s) of InstExecution/InstStep

src/ReactorModel/Execution/Basic.lean
@@ -10,18 +10,18 @@ noncomputable def schedule (act : Time.Tag ▸ Value) (t : Time) (v : Value) : T
   | some g => act.update ⟨t, g.microsteps + 1⟩ v
 
 inductive ChangeStep (rcn : ID) (s : State) : State → Change → Prop 
-  | port {σ' i v} :     (s.rtr -[Cmp.prt:i (⟨·.role, v⟩)]→ σ')    → ChangeStep rcn s ⟨σ', s.ctx⟩ (Change.port i v)
-  | state {σ' i v} :    (s.rtr -[Cmp.stv:i λ _ => v]→ σ')         → ChangeStep rcn s ⟨σ', s.ctx⟩ (Change.state i v)
-  | action {σ' i t v} : (s.rtr -[Cmp.act:i (schedule · t v)]→ σ') → ChangeStep rcn s ⟨σ', s.ctx⟩ (Change.action i t v)
-  -- | connect {σ' src dst r} :    (s.rtr &[Cmp.rcn:rcn]= r) → (s.rtr -[Cmp.rcn|r (·.update (s.freshID Cmp.rcn r) (Reaction.relay src dst))]→ σ') → ChangeStep rcn s ⟨σ', s.ctx⟩ (Change.connect src dst)
-  -- | disconnect {σ' src dst r} : (s.rtr &[Cmp.rcn:rcn]= r) → (s.rtr -[Cmp.rcn|r (·.filter' (· ≠ Reaction.relay src dst))]→ σ')                  → ChangeStep rcn s ⟨σ', s.ctx⟩ (Change.disconnect src dst)
+  | port {σ' i v} :     (s.rtr -[.prt:i (⟨·.role, v⟩)]→ σ')    → ChangeStep rcn s ⟨σ', s.ctx⟩ (.port i v)
+  | state {σ' i v} :    (s.rtr -[.stv:i λ _ => v]→ σ')         → ChangeStep rcn s ⟨σ', s.ctx⟩ (.state i v)
+  | action {σ' i t v} : (s.rtr -[.act:i (schedule · t v)]→ σ') → ChangeStep rcn s ⟨σ', s.ctx⟩ (.action i t v)
+  -- | connect {σ' src dst r} :    (s.rtr &[.rcn:rcn]= r) → (s.rtr -[Cmp.rcn|r (·.update (s.freshID Cmp.rcn r) (Reaction.relay src dst))]→ σ') → ChangeStep rcn s ⟨σ', s.ctx⟩ (.connect src dst)
+  -- | disconnect {σ' src dst r} : (s.rtr &[.rcn:rcn]= r) → (s.rtr -[Cmp.rcn|r (·.filter' (· ≠ Reaction.relay src dst))]→ σ')                  → ChangeStep rcn s ⟨σ', s.ctx⟩ (.disconnect src dst)
   -- TODO: `create` via reactor class instantiation function
-  -- | delete {σ' i r} :           (s.rtr &[Cmp.rcn:rcn]= r) → (s.rtr -[Cmp.rtr|r (·.update i none)]→ σ')                                         → ChangeStep rcn s ⟨σ', s.ctx⟩ (Change.delete i)
+  -- | delete {σ' i r} :           (s.rtr &[.rcn:rcn]= r) → (s.rtr -[Cmp.rtr|r (·.update i none)]→ σ')                                         → ChangeStep rcn s ⟨σ', s.ctx⟩ (.delete i)
   -- Mutations are (temporarily) no-ops:
-  | connect {i₁ i₂} :    ChangeStep rcn s s (Change.connect i₁ i₂)
-  | disconnect {i₁ i₂} : ChangeStep rcn s s (Change.disconnect i₁ i₂)
-  | create {rtr} :       ChangeStep rcn s s (Change.create rtr)
-  | delete {i} :         ChangeStep rcn s s (Change.delete i)
+  | connect {i₁ i₂} :    ChangeStep rcn s s (.connect i₁ i₂)
+  | disconnect {i₁ i₂} : ChangeStep rcn s s (.disconnect i₁ i₂)
+  | create {rtr} :       ChangeStep rcn s s (.create rtr)
+  | delete {i} :         ChangeStep rcn s s (.delete i)
 
 notation s₁:max " -[" rcn ":" c "]→ " s₂:max => ChangeStep rcn s₁ s₂ c
 
@@ -34,35 +34,34 @@ notation s₁:max " -[" rcn ":" cs "]→* " s₂:max => ChangeListStep rcn s₁ 
 -- We separate the execution into two parts, the instantaneous execution which controlls
 -- how reactors execute at a given instant, and the timed execution, which includes the
 -- passing of time
-inductive InstStep (s : State) : State → Prop 
-  | execReaction {rcn} {i : ID} {s'} : 
-    (s.rtr *[Cmp.rcn:i]= rcn) →
+inductive InstStep (s : State) (i : ID) : State → Prop 
+  | execReaction {rcn} {s'} : 
+    (s.rtr *[.rcn:i]= rcn) →
     (s.allows i) →
     (s.triggers rcn) →
     (s -[i:rcn (s.rcnInput rcn)]→* s') →
-    InstStep s ⟨s'.rtr, s'.ctx.addCurrentExecuted i⟩
-  | skipReaction {rcn} {i : ID} :
-    (s.rtr *[Cmp.rcn:i]= rcn) →
+    InstStep s i ⟨s'.rtr, s'.ctx.addCurrentProcessed i⟩
+  | skipReaction {rcn} :
+    (s.rtr *[.rcn:i]= rcn) →
     (s.allows i) →
     (¬ s.triggers rcn) →
-    InstStep s ⟨s.rtr, s.ctx.addCurrentExecuted i⟩
+    InstStep s i ⟨s.rtr, s.ctx.addCurrentProcessed i⟩
 
-notation s₁:max " ⇓ᵢ " s₂:max => InstStep s₁ s₂
+notation s₁:max " ⇓ᵢ[" rcn "] " s₂:max => InstStep s₁ rcn s₂
 
 -- An execution at an instant is a series of steps,
 -- which we model with the transitive closure.
-inductive InstExecution : State → State → Prop 
-  | single {s₁ s₂} : s₁ ⇓ᵢ s₂ → InstExecution s₁ s₂
-  | trans {s₁ s₂ s₃} : s₁ ⇓ᵢ s₂ → InstExecution s₂ s₃ → InstExecution s₁ s₃
+inductive InstExecution : State → List ID → State → Prop 
+  | single {s₁ rcn s₂} : s₁ ⇓ᵢ[rcn] s₂ → InstExecution s₁ [rcn] s₂
+  | trans {s₁ hd s₂ tl s₃} : s₁ ⇓ᵢ[hd] s₂ → InstExecution s₂ tl s₃ → InstExecution s₁ (hd::tl) s₃
 
-notation s₁:max " ⇓ᵢ+ " s₂:max => InstExecution s₁ s₂
+notation s₁:max " ⇓ᵢ+[" rcns "] " s₂:max => InstExecution s₁ rcns s₂
 
-abbrev State.instComplete (s : State) : Prop := s.ctx.currentExecutedRcns = s.rtr.ids Cmp.rcn
+abbrev State.instComplete (s : State) : Prop := s.ctx.currentProcessedRcns = s.rtr.ids Cmp.rcn
 
-structure CompleteInstExecution (s₁ s₂ : State) : Prop where
-  exec : s₁ ⇓ᵢ+ s₂
-  complete : s₂.instComplete
-
+inductive CompleteInstExecution (s₁ s₂ : State) : Prop
+  | mk : (rcns : List ID) → (s₁ ⇓ᵢ+[rcns] s₂) → s₂.instComplete → CompleteInstExecution s₁ s₂
+  
 notation s₁:max " ⇓ᵢ| " s₂:max => CompleteInstExecution s₁ s₂
 
 def clearingPorts (σ₁ σ₂ : Reactor) : Prop := sorry -- TODO: Define this via MultiUpdate if that is realized.
